libs

specs/lib/Spec.Lib.IntTypes.fst
@@ -1,53 +1,39 @@
 module Spec.Lib.IntTypes
 
 (* Declared in .fsti : intsize, bits, maxint *)
-#set-options "--z3rlimit 50"
+#set-options "--z3rlimit 10 --max_fuel 0"
 
-let uint_n (t:inttype) : Type0 = 
+let uint_t (t:inttype) : Type0 = 
   match t with
   | U8 -> UInt8.t
   | U16 -> UInt16.t
   | U32 -> UInt32.t
   | U64 -> UInt64.t
   | U128 -> UInt128.t
-    
-type uint_ =
- | UInt: t:inttype -> v:uint_n t -> uint_
 
-let uint = uint_
-let ty u = u.t
-type uint_t (t:inttype) = u:uint{ty u = t}
-let uint_to_nat_ (u:uint) = 
-  match u with
-  | UInt U8 x -> UInt8.v x
-  | UInt U16 x -> UInt16.v x
-  | UInt U32 x -> UInt32.v x
-  | UInt U64 x -> UInt64.v x
-  | UInt U128 x -> UInt128.v x
+let uint_to_nat_ #t (x:uint_t t) = 
+  match t with
+  | U8 -> UInt8.v x
+  | U16 -> UInt16.v x
+  | U32 -> UInt32.v x
+  | U64 -> UInt64.v x
+  | U128 -> UInt128.v x
 
 let uint_v #t u = uint_to_nat_ u
 
 (* Declared in .fsti: uint8, uint16, uint32, uint64, uint128 *)
 
-let u8 x : uint8 = 
-  UInt U8 (UInt8.uint_to_t x)
+let u8 x : uint8  = UInt8.uint_to_t x 
 
-let u8uy x = UInt U8 x
+let u8uy x = x
   
-let u8_ x : uint8 = 
-  UInt U8 (UInt8.uint_to_t x)
+let u16 x : uint16 = UInt16.uint_to_t x
 
-let u16 x : uint16 = 
-  UInt U16 (UInt16.uint_to_t x)
+let u32 x : uint32 = UInt32.uint_to_t x
 
-let u32 x : uint32 = 
-  UInt U32 (UInt32.uint_to_t x)
+let u64 x : uint64 = UInt64.uint_to_t x
 
-let u64 x : uint64 = 
-  UInt U64 (UInt64.uint_to_t x)
-
-let u128 x : uint128 = 
-  UInt U128 (UInt128.uint_to_t x)
+let u128 x : uint128 = UInt128.uint_to_t x
 
 let uint_to_nat #t u = uint_to_nat_ u
 let nat_to_uint #t x : uint_t t = 
@@ -64,181 +50,181 @@ let cast #t u t' =
   nat_to_uint #t' n'
   
 let add_mod #t a b =
-  match a,b with
-  | UInt U8 a, UInt U8 b -> UInt U8 (UInt8.add_mod a b)
-  | UInt U16 a, UInt U16 b -> UInt U16 (UInt16.add_mod a b)
-  | UInt U32 a, UInt U32 b -> UInt U32 (UInt32.add_mod a b)
-  | UInt U64 a, UInt U64 b -> UInt U64 (UInt64.add_mod a b)
-  | UInt U128 a, UInt U128 b -> UInt U128 (UInt128.add_mod a b)
+  match t with
+  | U8  -> (UInt8.add_mod a b)
+  | U16 -> (UInt16.add_mod a b)
+  | U32 -> (UInt32.add_mod a b)
+  | U64 -> (UInt64.add_mod a b)
+  | U128 -> (UInt128.add_mod a b)
   
 
 let add #t a b = 
-  match a,b with
-  | UInt U8 a, UInt U8 b -> UInt U8 (UInt8.add a b)
-  | UInt U16 a, UInt U16 b -> UInt U16 (UInt16.add a b)
-  | UInt U32 a, UInt U32 b -> UInt U32 (UInt32.add a b)
-  | UInt U64 a, UInt U64 b -> UInt U64 (UInt64.add a b)
-  | UInt U128 a, UInt U128 b -> UInt U128 (UInt128.add a b)
+  match t with
+  | U8 -> (UInt8.add a b)
+  | U16 -> (UInt16.add a b)
+  | U32 -> (UInt32.add a b)
+  | U64 -> (UInt64.add a b)
+  | U128 -> (UInt128.add a b)
 
 let incr #t a = 
-  match a with
-  | UInt U8 a -> UInt U8 (UInt8.add a 0x1uy)
-  | UInt U16 a -> UInt U16 (UInt16.add a 0x1us)
-  | UInt U32 a -> UInt U32 (UInt32.add a 0x1ul)
-  | UInt U64 a -> UInt U64 (UInt64.add a 0x1uL)
-  | UInt U128 a -> UInt U128 (UInt128.add a (UInt128.uint_to_t 1))
+  match t with
+  | U8 -> (UInt8.add a 0x1uy)
+  | U16 -> (UInt16.add a 0x1us)
+  | U32 -> (UInt32.add a 0x1ul)
+  | U64 -> (UInt64.add a 0x1uL)
+  | U128 -> (UInt128.add a (UInt128.uint_to_t 1))
 
 
 
 let mul_mod #t a b = 
-  match a,b with
-  | UInt U8 a, UInt U8 b -> UInt U8 (UInt8.mul_mod a b)
-  | UInt U16 a, UInt U16 b -> UInt U16 (UInt16.mul_mod a b)
-  | UInt U32 a, UInt U32 b -> UInt U32 (UInt32.mul_mod a b)
-  | UInt U64 a, UInt U64 b -> UInt U64 (UInt64.mul_mod a b)
+  match t with
+  | U8 -> (UInt8.mul_mod a b)
+  | U16 -> (UInt16.mul_mod a b)
+  | U32 -> (UInt32.mul_mod a b)
+  | U64 -> (UInt64.mul_mod a b)
 
 
 let mul #t a b = 
-  match a,b with
-  | UInt U8 a, UInt U8 b -> UInt U8 (UInt8.mul a b)
-  | UInt U16 a, UInt U16 b -> UInt U16 (UInt16.mul a b)
-  | UInt U32 a, UInt U32 b -> UInt U32 (UInt32.mul a b)
-  | UInt U64 a, UInt U64 b -> UInt U64 (UInt64.mul a b)
+  match t with
+  | U8 -> (UInt8.mul a b)
+  | U16 -> (UInt16.mul a b)
+  | U32 -> (UInt32.mul a b)
+  | U64 -> (UInt64.mul a b)
 
 
 let sub_mod #t a b = 
-  match a,b with
-  | UInt U8 a, UInt U8 b -> UInt U8 (UInt8.sub_mod a b)
-  | UInt U16 a, UInt U16 b -> UInt U16 (UInt16.sub_mod a b)
-  | UInt U32 a, UInt U32 b -> UInt U32 (UInt32.sub_mod a b)
-  | UInt U64 a, UInt U64 b -> UInt U64 (UInt64.sub_mod a b)
-  | UInt U128 a, UInt U128 b -> UInt U128 (UInt128.sub_mod a b)
+  match t with
+  | U8 -> (UInt8.sub_mod a b)
+  | U16 -> (UInt16.sub_mod a b)
+  | U32 -> (UInt32.sub_mod a b)
+  | U64 -> (UInt64.sub_mod a b)
+  | U128 -> (UInt128.sub_mod a b)
 
 
 let sub #t a b = 
-  match a,b with
-  | UInt U8 a, UInt U8 b -> UInt U8 (UInt8.sub a b)
-  | UInt U16 a, UInt U16 b -> UInt U16 (UInt16.sub a b)
-  | UInt U32 a, UInt U32 b -> UInt U32 (UInt32.sub a b)
-  | UInt U64 a, UInt U64 b -> UInt U64 (UInt64.sub a b)
-  | UInt U128 a, UInt U128 b -> UInt U128 (UInt128.sub a b)
+  match t with
+  | U8 -> (UInt8.sub a b)
+  | U16 -> (UInt16.sub a b)
+  | U32 -> (UInt32.sub a b)
+  | U64 -> (UInt64.sub a b)
+  | U128 -> (UInt128.sub a b)
 
 let decr #t a = 
-  match a with
-  | UInt U8 a -> UInt U8 (UInt8.sub a 0x1uy)
-  | UInt U16 a -> UInt U16 (UInt16.sub a 0x1us)
-  | UInt U32 a -> UInt U32 (UInt32.sub a 0x1ul)
-  | UInt U64 a -> UInt U64 (UInt64.sub a 0x1uL)
-  | UInt U128 a -> UInt U128 (UInt128.sub a (UInt128.uint_to_t 1))
+  match t with
+  | U8 -> (UInt8.sub a 0x1uy)
+  | U16 -> (UInt16.sub a 0x1us)
+  | U32 -> (UInt32.sub a 0x1ul)
+  | U64 -> (UInt64.sub a 0x1uL)
+  | U128 -> (UInt128.sub a (UInt128.uint_to_t 1))
 
 let logxor #t a b = 
-  match a,b with
-  | UInt U8 a, UInt U8 b -> UInt U8 (UInt8.logxor a b)
-  | UInt U16 a, UInt U16 b -> UInt U16 (UInt16.logxor a b)
-  | UInt U32 a, UInt U32 b -> UInt U32 (UInt32.logxor a b)
-  | UInt U64 a, UInt U64 b -> UInt U64 (UInt64.logxor a b)
-  | UInt U128 a, UInt U128 b -> UInt U128 (UInt128.logxor a b)
+  match t with
+  | U8 -> (UInt8.logxor a b)
+  | U16 -> (UInt16.logxor a b)
+  | U32 -> (UInt32.logxor a b)
+  | U64 -> (UInt64.logxor a b)
+  | U128 -> (UInt128.logxor a b)
 
 
 let logand #t a b = 
-  match a,b with
-  | UInt U8 a, UInt U8 b -> UInt U8 (UInt8.logand a b)
-  | UInt U16 a, UInt U16 b -> UInt U16 (UInt16.logand a b)
-  | UInt U32 a, UInt U32 b -> UInt U32 (UInt32.logand a b)
-  | UInt U64 a, UInt U64 b -> UInt U64 (UInt64.logand a b)
-  | UInt U128 a, UInt U128 b -> UInt U128 (UInt128.logand a b)
+  match t with
+  | U8 -> (UInt8.logand a b)
+  | U16 -> (UInt16.logand a b)
+  | U32 -> (UInt32.logand a b)
+  | U64 -> (UInt64.logand a b)
+  | U128 -> (UInt128.logand a b)
 
 
 let logor #t a b = 
-  match a,b with
-  | UInt U8 a, UInt U8 b -> UInt U8 (UInt8.logor a b)
-  | UInt U16 a, UInt U16 b -> UInt U16 (UInt16.logor a b)
-  | UInt U32 a, UInt U32 b -> UInt U32 (UInt32.logor a b)
-  | UInt U64 a, UInt U64 b -> UInt U64 (UInt64.logor a b)
-  | UInt U128 a, UInt U128 b -> UInt U128 (UInt128.logor a b)
+  match t with
+  | U8 -> (UInt8.logor a b)
+  | U16 -> (UInt16.logor a b)
+  | U32 -> (UInt32.logor a b)
+  | U64 -> (UInt64.logor a b)
+  | U128 -> (UInt128.logor a b)
 
 
 let lognot #t a = 
-  match a with
-  | UInt U8 a -> UInt U8 (UInt8.lognot a)
-  | UInt U16 a -> UInt U16 (UInt16.lognot a)
-  | UInt U32 a -> UInt U32 (UInt32.lognot a)
-  | UInt U64 a -> UInt U64 (UInt64.lognot a)
-  | UInt U128 a -> UInt U128 (UInt128.lognot a)
+  match t with
+  | U8 -> (UInt8.lognot a)
+  | U16 -> (UInt16.lognot a)
+  | U32 -> (UInt32.lognot a)
+  | U64 -> (UInt64.lognot a)
+  | U128 -> (UInt128.lognot a)
 
 
 let shift_right #t a b = 
-  match a with
-  | UInt U8 a -> UInt U8 (UInt8.shift_right a b.v)
-  | UInt U16 a -> UInt U16 (UInt16.shift_right a b.v)
-  | UInt U32 a -> UInt U32 (UInt32.shift_right a b.v)
-  | UInt U64 a -> UInt U64 (UInt64.shift_right a b.v)
-  | UInt U128 a -> UInt U128 (UInt128.shift_right a b.v)
+  match t with
+  | U8 -> (UInt8.shift_right a b)
+  | U16 -> (UInt16.shift_right a b)
+  | U32 -> (UInt32.shift_right a b)
+  | U64 -> (UInt64.shift_right a b)
+  | U128 -> (UInt128.shift_right a b)
 
 
 let shift_left #t a b = 
-  match a with
-  | UInt U8 a -> UInt U8 (UInt8.shift_left a b.v)
-  | UInt U16 a -> UInt U16 (UInt16.shift_left a b.v)
-  | UInt U32 a -> UInt U32 (UInt32.shift_left a b.v)
-  | UInt U64 a -> UInt U64 (UInt64.shift_left a b.v)
-  | UInt U128 a -> UInt U128 (UInt128.shift_left a b.v)
+  match t with
+  | U8 -> (UInt8.shift_left a b)
+  | U16 -> (UInt16.shift_left a b)
+  | U32 -> (UInt32.shift_left a b)
+  | U64 -> (UInt64.shift_left a b)
+  | U128 -> (UInt128.shift_left a b)
 
 
 let rotate_right #t a b = 
-  (logor (shift_right a b)  (shift_left a (sub (u32 (bits a.t)) b)))
+  (logor (shift_right a b)  (shift_left a (sub #U32 (u32 (bits t)) b)))
 
 let rotate_left #t a b = 
-  (logor (shift_left a b)  (shift_right a (sub (u32 (bits a.t)) b)))
+  (logor (shift_left a b)  (shift_right a (sub #U32 (u32 (bits t)) b)))
 
 let eq_mask #t a b = 
-  match a,b with
-  | UInt U8 a, UInt U8 b -> if FStar.UInt8.(a =^ b) then (u8 (maxint U8)) else (u8 0)
-  | UInt U16 a, UInt U16 b -> if FStar.UInt16.(a =^ b) then (u16 (maxint U16)) else (u16 0)
-  | UInt U32 a, UInt U32 b -> if FStar.UInt32.(a =^ b) then (u32 (maxint U32)) else (u32 0) 
-  | UInt U64 a, UInt U64 b -> if FStar.UInt64.(a =^ b) then (u64 (maxint U64)) else (u64 0) 
-  | UInt U128 a, UInt U128 b -> if FStar.UInt128.(a =^ b) then (u128 (maxint U128)) else (u128 0)
+  match t with
+  | U8 -> if FStar.UInt8.(a =^ b) then (u8 (maxint U8)) else (u8 0)
+  | U16 -> if FStar.UInt16.(a =^ b) then (u16 (maxint U16)) else (u16 0)
+  | U32 -> if FStar.UInt32.(a =^ b) then (u32 (maxint U32)) else (u32 0) 
+  | U64 -> if FStar.UInt64.(a =^ b) then (u64 (maxint U64)) else (u64 0) 
+  | U128 -> if FStar.UInt128.(a =^ b) then (u128 (maxint U128)) else (u128 0)
 
 let neq_mask #t a b = 
-  match a,b with
-  | UInt U8 a, UInt U8 b -> if not FStar.UInt8.(a =^ b) then (u8 (maxint U8)) else (u8 0)
-  | UInt U16 a, UInt U16 b -> if not FStar.UInt16.(a =^ b) then (u16 (maxint U16)) else (u16 0)
-  | UInt U32 a, UInt U32 b -> if not FStar.UInt32.(a =^ b) then (u32 (maxint U32)) else (u32 0) 
-  | UInt U64 a, UInt U64 b -> if not FStar.UInt64.(a =^ b) then (u64 (maxint U64)) else (u64 0) 
-  | UInt U128 a, UInt U128 b -> if not FStar.UInt128.(a =^ b) then (u128 (maxint U128)) else (u128 0)
+  match t with
+  | U8 -> if not FStar.UInt8.(a =^ b) then (u8 (maxint U8)) else (u8 0)
+  | U16 -> if not FStar.UInt16.(a =^ b) then (u16 (maxint U16)) else (u16 0)
+  | U32 -> if not FStar.UInt32.(a =^ b) then (u32 (maxint U32)) else (u32 0) 
+  | U64 -> if not FStar.UInt64.(a =^ b) then (u64 (maxint U64)) else (u64 0) 
+  | U128 -> if not FStar.UInt128.(a =^ b) then (u128 (maxint U128)) else (u128 0)
 
 let gte_mask #t a b = 
-  match a,b with
-  | UInt U8 a, UInt U8 b -> if FStar.UInt8.(a >=^ b) then (u8 (maxint U8)) else (u8 0)
-  | UInt U16 a, UInt U16 b -> if FStar.UInt16.(a >=^ b) then (u16 (maxint U16)) else (u16 0)
-  | UInt U32 a, UInt U32 b -> if FStar.UInt32.(a >=^ b) then (u32 (maxint U32)) else (u32 0) 
-  | UInt U64 a, UInt U64 b -> if FStar.UInt64.(a >=^ b) then (u64 (maxint U64)) else (u64 0) 
-  | UInt U128 a, UInt U128 b -> if FStar.UInt128.(a >=^ b) then (u128 (maxint U128)) else (u128 0)
+  match t with
+  | U8 -> if FStar.UInt8.(a >=^ b) then (u8 (maxint U8)) else (u8 0)
+  | U16 -> if FStar.UInt16.(a >=^ b) then (u16 (maxint U16)) else (u16 0)
+  | U32 -> if FStar.UInt32.(a >=^ b) then (u32 (maxint U32)) else (u32 0) 
+  | U64 -> if FStar.UInt64.(a >=^ b) then (u64 (maxint U64)) else (u64 0) 
+  | U128 -> if FStar.UInt128.(a >=^ b) then (u128 (maxint U128)) else (u128 0)
 
 let gt_mask #t a b = 
-  match a,b with
-  | UInt U8 a, UInt U8 b -> if FStar.UInt8.(a >^ b) then (u8 (maxint U8)) else (u8 0)
-  | UInt U16 a, UInt U16 b -> if FStar.UInt16.(a >^ b) then (u16 (maxint U16)) else (u16 0)
-  | UInt U32 a, UInt U32 b -> if FStar.UInt32.(a >^ b) then (u32 (maxint U32)) else (u32 0) 
-  | UInt U64 a, UInt U64 b -> if FStar.UInt64.(a >^ b) then (u64 (maxint U64)) else (u64 0) 
-  | UInt U128 a, UInt U128 b -> if FStar.UInt128.(a >^ b) then (u128 (maxint U128)) else (u128 0)
+  match t with
+  | U8 -> if FStar.UInt8.(a >^ b) then (u8 (maxint U8)) else (u8 0)
+  | U16 -> if FStar.UInt16.(a >^ b) then (u16 (maxint U16)) else (u16 0)
+  | U32 -> if FStar.UInt32.(a >^ b) then (u32 (maxint U32)) else (u32 0) 
+  | U64 -> if FStar.UInt64.(a >^ b) then (u64 (maxint U64)) else (u64 0) 
+  | U128 -> if FStar.UInt128.(a >^ b) then (u128 (maxint U128)) else (u128 0)
 
 
 let lt_mask #t a b = 
-  match a,b with
-  | UInt U8 a, UInt U8 b -> if FStar.UInt8.(a <^ b) then (u8 (maxint U8)) else (u8 0)
-  | UInt U16 a, UInt U16 b -> if FStar.UInt16.(a <^ b) then (u16 (maxint U16)) else (u16 0)
-  | UInt U32 a, UInt U32 b -> if FStar.UInt32.(a <^ b) then (u32 (maxint U32)) else (u32 0) 
-  | UInt U64 a, UInt U64 b -> if FStar.UInt64.(a <^ b) then (u64 (maxint U64)) else (u64 0) 
-  | UInt U128 a, UInt U128 b -> if FStar.UInt128.(a <^ b) then (u128 (maxint U128)) else (u128 0)
+  match t with
+  | U8 -> if FStar.UInt8.(a <^ b) then (u8 (maxint U8)) else (u8 0)
+  | U16 -> if FStar.UInt16.(a <^ b) then (u16 (maxint U16)) else (u16 0)
+  | U32 -> if FStar.UInt32.(a <^ b) then (u32 (maxint U32)) else (u32 0) 
+  | U64 -> if FStar.UInt64.(a <^ b) then (u64 (maxint U64)) else (u64 0) 
+  | U128 -> if FStar.UInt128.(a <^ b) then (u128 (maxint U128)) else (u128 0)
 
 let lte_mask #t a b = 
-  match a,b with
-  | UInt U8 a, UInt U8 b -> if FStar.UInt8.(a <=^ b) then (u8 (maxint U8)) else (u8 0)
-  | UInt U16 a, UInt U16 b -> if FStar.UInt16.(a <=^ b) then (u16 (maxint U16)) else (u16 0)
-  | UInt U32 a, UInt U32 b -> if FStar.UInt32.(a <=^ b) then (u32 (maxint U32)) else (u32 0) 
-  | UInt U64 a, UInt U64 b -> if FStar.UInt64.(a <=^ b) then (u64 (maxint U64)) else (u64 0) 
-  | UInt U128 a, UInt U128 b -> if FStar.UInt128.(a <=^ b) then (u128 (maxint U128)) else (u128 0)
+  match t with
+  | U8 -> if FStar.UInt8.(a <=^ b) then (u8 (maxint U8)) else (u8 0)
+  | U16 -> if FStar.UInt16.(a <=^ b) then (u16 (maxint U16)) else (u16 0)
+  | U32 -> if FStar.UInt32.(a <=^ b) then (u32 (maxint U32)) else (u32 0) 
+  | U64 -> if FStar.UInt64.(a <=^ b) then (u64 (maxint U64)) else (u64 0) 
+  | U128 -> if FStar.UInt128.(a <=^ b) then (u128 (maxint U128)) else (u128 0)
  
 (* defined in .fsti: notations +^, -^, ...*)
 
@@ -258,3 +244,5 @@ let bn_div a b = a / b
 
 
   
+
+
